@prefix rdf: <http://www.w3.org/1999/02/22-rdf-syntax-ns#> .
@prefix rdfs: <http://www.w3.org/2000/01/rdf-schema#> .
@prefix : <http://www.w3.org/2000/01/rdf-schema#> .
@prefix dc: <http://purl.org/dc/elements/1.1/> .
@prefix owl: <http://www.w3.org/2002/07/owl#> .
@prefix prov: <http://www.w3.org/ns/prov#> .
@prefix dgb: <https://discoursegraphs.com/schema/dg_base#> .
@prefix dg: <https://discoursegraphs.com/schema/dg_core#> .
# http://purl.org/spar/po
@prefix po: <http://www.essepuntato.it/2008/12/pattern#> .

<https://discoursegraphs.com/schema/dg_core#>
    dc:date "2025-12-31" ;
    rdfs:comment "DiscourseGraph core vocabulary"@en ;
    rdfs:label "DiscourseGraph core vocabulary"@en ;
    owl:versionInfo "0 (tentative)" ;
    a owl:Ontology.

dg:Question a dgb:NodeSchema;
  rdfs:label "Question"@en;
  rdfs:comment "Scientific unknowns that we want to make known, and are addressable by the systematic application of research methods"@en.

dg:Claim a dgb:NodeSchema;
  rdfs:label "Claim"@en;
  rdfs:comment "Atomic, generalized assertions about the world that (propose to) answer research questions"@en.

dg:Evidence a dgb:NodeSchema;
  rdfs:label "Evidence"@en;
  rdfs:comment "A specific empirical observation from a particular application of a research method"@en.

dg:Source a dgb:NodeSchema;
  rdfs:label "Source"@en;
  rdfs:comment "Some research source that reports/generates evidence, like an experiment/study, book, conference paper, or journal article"@en.

dg:opposesCE a dgb:RelationDef;
  rdfs:label "Opposes"@en;
  rdfs:range dg:Claim;
  rdfs:domain dg:Evidence.

dg:opposedByEC a dgb:RelationDef;
  rdfs:label "Opposed by"@en;
  owl:inverseOf dg:opposesCE;
  rdfs:range dg:Evidence;
  rdfs:domain dg:Claim.

dg:supportsCE a dgb:RelationDef;
  rdfs:label "Supports"@en;
  rdfs:range dg:Claim;
  rdfs:domain dg:Evidence.

dg:supportedByEC a dgb:RelationDef;
  rdfs:label "Supported by"@en;
  owl:inverseOf dg:supportsCE;
  rdfs:range dg:Evidence;
  rdfs:domain dg:Claim.

dg:opposesCC a dgb:RelationDef;
  rdfs:label "Opposes"@en;
  rdfs:range dg:Claim;
  rdfs:domain dg:Claim.

dg:opposedByCC a dgb:RelationDef;
  rdfs:label "Opposed by"@en;
  owl:inverseOf dg:opposesCC;
  rdfs:range dg:Claim;
  rdfs:domain dg:Claim.

dg:supportsCC a dgb:RelationDef;
  rdfs:label "Supports"@en;
  rdfs:range dg:Claim;
  rdfs:domain dg:Claim.

dg:supportedByCC a dgb:RelationDef;
  rdfs:label "Supported by"@en;
  owl:inverseOf dg:supportsCC;
  rdfs:range dg:Claim;
  rdfs:domain dg:Claim.

dg:addresses a dgb:RelationDef;
  rdfs:label "Addresses"@en;
  rdfs:range dg:Question;
  rdfs:domain dg:Claim.

dg:addressedBy a dgb:RelationDef;
  rdfs:label "Addressed by"@en;
  owl:inverseOf dg:addresses;
  rdfs:range dg:Claim;
  rdfs:domain dg:Question.

dg:curatedTo a dgb:RelationDef;
  rdfs:label "Curated to"@en;
  rdfs:range dg:Source;
  rdfs:domain dg:Evidence.

dg:curatedFrom a dgb:RelationDef;
  owl:inverseOf dg:curatedTo;
  rdfs:label "Curated from"@en;
  rdfs:range dg:Evidence;
  rdfs:domain dg:Source.

dg:containsRec a owl:TransitiveProperty.
po:contains rdfs:subClassOf dg:containsRec.
dct:hasPart rdfs:subClassOf dg:containsRec.

dg:containsRef a owl:ObjectProperty;
  owl:propertyChainAxiom (dg:containsRec dct:references);
  rdfs:label "Contains a reference to"@en.

dg:backlink a owl:ObjectProperty;
  owl:inverseOf dg:containsRef;
  rdfs:label "is referred by"@en.
